Split cat example files into two parts
First is catfileSystem: this has material that is independent of cf and
the translator.  Second is cat, which brings in the cf tech.

compiler/bootstrap/io/catfileSystemScript.sml
@@ -1,13 +1,13 @@
 open preamble
 
-open ml_translatorTheory ml_translatorLib semanticPrimitivesTheory
-open cfHeapsTheory cfTheory cfTacticsBaseLib cfTacticsLib ml_progLib
 open monadsyntax
 
 val _ = new_theory "catfileSystem";
 
 val _ = overload_on ("return", ``SOME``)
 val _ = overload_on ("fail", ``NONE``)
+val _ = overload_on ("SOME", ``SOME``)
+val _ = overload_on ("NONE", ``NONE``)
 val _ = overload_on ("monad_bind", ``OPTION_BIND``)
 val _ = overload_on ("monad_unit_bind", ``OPTION_IGNORE_BIND``)
 
@@ -258,337 +258,27 @@ val write_lemma = Q.store_thm(
      SOME ([c], encode (fs with stdout := fs.stdout ++ [CHR (w2n c)]))`,
   simp[fs_ffi_next_def, decode_encode_FS, writeStdOut_def]);
 
-(* ----------------------------------------------------------------------
-
-    Our operations require memory to be allocated in the heap for the
-    passing of parameters:
-
-    1. write requires write_loc for the storage of the character to be
-       written
-    2. open-file requires filenamae_loc for the storage of the name of the
-       (probably zero-terminated) file
-    3. read-char needs storage for a single byte for identifying the
-       file-descripter to read through. This assumes that there can't
-       be more than 256 file-descriptors.  Perhaps we can share write_loc.
-    4. close-file also needs a file-descriptor.
-
-    Memory of this sort can be pre-allocated by making calls to AST
-    expressions like
-
-      App Aw8alloc [Lit (IntLit sz); Lit (Word8 0w)]
-
-    where sz is the number of bytes needed.
-
-   ---------------------------------------------------------------------- *)
-
-(* first copy the Word8Array and CHAR_IO set up from helloProg, adding an
-   extra array for filenames, of length FILENAME_MAX
-*)
-(* setup *)
-
-fun get_module_prefix () = let
-  val mod_tm = ml_progLib.get_thm (get_ml_prog_state ())
-               |> concl |> rator |> rator |> rand
-  in if optionSyntax.is_none mod_tm then "" else
-       stringSyntax.fromHOLstring (mod_tm |> rand |> rator |> rand) ^ "_"
-  end
-
-fun trans ml_name q = let
-  val rhs = Term q
-  val prefix = get_module_prefix ()
-  val tm = mk_eq(mk_var(prefix ^ pick_name ml_name,type_of rhs),rhs)
-  val def = Define `^tm`
-  val _ = (next_ml_names := [ml_name])
-  val v_thm = translate (def |> SIMP_RULE std_ss [FUN_EQ_THM])
-  val v_thm = v_thm |> REWRITE_RULE [def]
-                    |> CONV_RULE (DEPTH_CONV ETA_CONV)
-  val v_name = v_thm |> concl |> rand |> dest_const |> fst
-  (* evaluate precondition *)
-  val pat = PRECONDITION_def |> SPEC_ALL |> GSYM |> concl |> rand
-  fun PRECOND_CONV c tm =
-    if can (match_term pat) tm then RAND_CONV c tm else NO_CONV tm
-  val v_thm = v_thm |> DISCH_ALL
-                    |> CONV_RULE (ONCE_DEPTH_CONV (PRECOND_CONV EVAL))
-                    |> UNDISCH_ALL
-  val _ = save_thm(v_name ^ "_thm",v_thm)
-  in v_thm end
-
-fun append_prog tm = let
-  val tm = QCONV EVAL tm |> concl |> rand
-  in ml_prog_update (ml_progLib.add_prog tm pick_name) end
-
-fun append_dec tm = let
-  val tm = QCONV EVAL tm |> concl |> rand
-  in ml_prog_update (ml_progLib.add_dec tm pick_name) end
-
-fun append_decs tm = let
-  val tm = QCONV EVAL tm |> concl |> rand
-  val tms = fst (listSyntax.dest_list tm)
-  in (map append_dec tms; ()) end
-
-fun basis_st () = get_ml_prog_state ()
-
-val _ = Define `
-  mk_binop name prim = Dlet (Pvar name)
-    (Fun "x" (Fun "y" (App prim [Var (Short "x"); Var (Short "y")])))`;
-
-val _ = Define `
-  mk_unop name prim = Dlet (Pvar name)
-    (Fun "x" (App prim [Var (Short "x")]))`;
-
-
-
-(* Word8Array module -- CF verified *)
-
-val _ = ml_prog_update (open_module "Word8Array");
-
-val _ = append_decs
-   ``[mk_binop "array" Aw8alloc;
-      mk_binop "sub" Aw8sub;
-      mk_unop "length" Aw8length;
-      Dlet (Pvar "update") (Fun "x" (Fun "y" (Fun "z"
-        (App Aw8update [Var (Short "x"); Var (Short "y"); Var (Short "z")])))) ]``
-
-val _ = ml_prog_update (close_module NONE);
-
-fun prove_array_spec op_name =
-  xcf op_name (basis_st()) \\ TRY xpull \\
-  fs [cf_aw8alloc_def, cf_aw8sub_def, cf_aw8length_def, cf_aw8update_def,
-      cf_aalloc_def, cf_asub_def, cf_alength_def, cf_aupdate_def] \\
-  irule local_elim \\ reduce_tac \\
-  fs [app_aw8alloc_def, app_aw8sub_def, app_aw8length_def, app_aw8update_def,
-      app_aalloc_def, app_asub_def, app_alength_def, app_aupdate_def] \\
-  xsimpl \\ fs [INT_def, NUM_def, WORD_def, w2w_def, UNIT_TYPE_def] \\
-  TRY (simp_tac (arith_ss ++ intSimps.INT_ARITH_ss) [])
-
-val w8array_alloc_spec = store_thm ("w8array_alloc_spec",
-  ``!n nv w wv.
-     NUM n nv /\ WORD w wv ==>
-     app (p:'ffi ffi_proj) ^(fetch_v "Word8Array.array" (basis_st())) [nv; wv]
-       emp (POSTv v. W8ARRAY v (REPLICATE n w))``,
-  prove_array_spec "Word8Array.array");
-
-val w8array_sub_spec = store_thm ("w8array_sub_spec",
-  ``!a av n nv.
-     NUM n nv /\ n < LENGTH a ==>
-     app (p:'ffi ffi_proj) ^(fetch_v "Word8Array.sub" (basis_st())) [av; nv]
-       (W8ARRAY av a) (POSTv v. cond (WORD (EL n a) v) * W8ARRAY av a)``,
-  prove_array_spec "Word8Array.sub");
-
-val w8array_length_spec = store_thm ("w8array_length_spec",
-  ``!a av.
-     app (p:'ffi ffi_proj) ^(fetch_v "Word8Array.length" (basis_st())) [av]
-       (W8ARRAY av a) (POSTv v. cond (NUM (LENGTH a) v) * W8ARRAY av a)``,
-  prove_array_spec "Word8Array.length");
-
-val w8array_update_spec = store_thm ("w8array_update_spec",
-  ``!a av n nv w wv.
-     NUM n nv /\ n < LENGTH a /\ WORD w wv ==>
-     app (p:'ffi ffi_proj) ^(fetch_v "Word8Array.update" (basis_st()))
-       [av; nv; wv]
-       (W8ARRAY av a)
-       (POSTv v. cond (UNIT_TYPE () v) * W8ARRAY av (LUPDATE w n a))``,
-  prove_array_spec "Word8Array.update");
-
-
-(* CharIO -- CF verified *)
-
-val _ = ml_prog_update (open_module "CharIO");
-
-fun derive_eval_thm v_name e = let
-  val th = get_ml_prog_state () |> get_thm
-  val th = MATCH_MP ml_progTheory.ML_code_NONE_Dlet_var th
-           handle HOL_ERR _ =>
-           MATCH_MP ml_progTheory.ML_code_SOME_Dlet_var th
-  val goal = th |> SPEC e |> SPEC_ALL |> concl |> dest_imp |> fst
-  val lemma = goal
-    |> (NCONV 50 (SIMP_CONV (srw_ss()) [Once bigStepTheory.evaluate_cases,
-            PULL_EXISTS,do_app_def,store_alloc_def,LET_THM]) THENC EVAL)
-  val v_thm = prove(mk_imp(lemma |> concl |> rand,goal),fs [lemma])
-                 |> GEN_ALL |> SIMP_RULE std_ss [] |> SPEC_ALL
-  val v_tm = v_thm |> concl |> rand |> rand |> rand
-  val v_def = define_abbrev true v_name v_tm
-  in v_thm |> REWRITE_RULE [GSYM v_def] end
-
-val onechar_e = ``(App Aw8alloc [Lit (IntLit 1); Lit (Word8 0w)])``
-val filename_e = ``(App Aw8alloc [Lit (IntLit 256); Lit (Word8 0w)])``
-
-(*
-   - onechar_loc is the name of the HOL constant
-   - onechar is the name of the binding in the module
-*)
-val _ = ml_prog_update
-          (add_Dlet (derive_eval_thm "onechar_loc" onechar_e) "onechar" [])
-
-(* similarly
-   - filename_loc is the name of the HOL constant
-   - filename_array is the name of the binding in the module
-*)
-val _ = ml_prog_update
-          (add_Dlet
-             (derive_eval_thm "filename_loc" filename_e)
-             "filename_array"
-             [])
-
-
-(* TODO: these two can definitely move somewhere else *)
-val Apps_def = tDefine "Apps" `
-  (Apps [x;y] = App Opapp [x;y]) /\
-  (Apps [] = ARB) /\
-  (Apps xs = App Opapp [Apps (FRONT xs); LAST xs])`
-  (WF_REL_TAC `measure LENGTH` \\ fs [LENGTH_FRONT]);
-
-val LetApps_def = Define `
-  LetApps n f args = Let (SOME n) (Apps (Var f::args))`;
-
-(* ML implementation of write function (0), with parameter "c" *)
-val write_e =
-  ``LetApps "c" (Long "Word8Array" "update")
-                [Var (Short "onechar"); Lit (IntLit 0); Var (Short "c")]
-        (Let (SOME "_") (App (FFI 0) [Var (Short "onechar")])
-             (Var (Short "c")))``
-  |> EVAL |> concl |> rand
-val _ = ml_prog_update (add_Dlet_Fun ``"write"`` ``"c"`` write_e "write_v")
-
-(* ML implementation of open function (1), with parameter name "fname" *)
-val open_e =
-  ``Let (SOME "_")
-        (Apps [Var (Long "Word8Array" "copyVec");
-               Var (Short "filename_array");
-               Var (Short "fname")])
-        (App (FFI 1) [Var (Short "filename_array")])`` |> EVAL |> concl |> rand
-val _ = ml_prog_update (add_Dlet_Fun ``"open"`` ``"fname"`` open_e "open_v")
-val open_v_def = definition "open_v_def"
-
-(* ML implementation of fgetc function (2), with parameter name "fd" *)
-val fgetc_e =
-  ``Let (SOME "_")
-        (Apps [Var (Long "Word8Array" "update");
-               Var (Short "onechar");
-               Lit (IntLit 0);
-               Var (Short "fd")])
-        (App (FFI 2) [Var (Short "onechar")])`` |> EVAL |> concl |> rand
-val _ = ml_prog_update (add_Dlet_Fun ``"fgetc"`` ``"fd"`` fgetc_e "fgetc_v")
-val fgetc_v_def = definition "fgetc_v_def"
-
-(* ML implementation of close function (3), with parameter "w8" *)
-val close_e =
-  ``Let (SOME "_") (Apps [Var (Long "Word8Array" "update");
-                          Var (Short "onechar");
-                          Lit (IntLit 0);
-                          Var (Short "w8")])
-             (Let (SOME "_") (App (FFI 3) [Var (Short "onechar")])
-                  (Con NONE []))`` |> EVAL |> concl |> rand
-val _ = ml_prog_update (add_Dlet_Fun ``"close"`` ``"w8"`` close_e "close_v")
-
-val _ = ml_prog_update (close_module NONE);
-
-val CATFS_def = Define `
-  CATFS fs = IO (encode fs) fs_ffi_next [0;1;2;3]`
-
-val CHAR_IO_char1_def = Define `
-  CHAR_IO_char1 = SEP_EXISTS w. W8ARRAY onechar_loc [w]`;
-
-val CHAR_IO_fname_def = Define`
-  CHAR_IO_fname = SEP_EXISTS v. W8ARRAY filename_loc v * cond (LENGTH v = 256)
+(* insert null-terminated-string (l1) at specified index (n) in a list (l2) *)
+val insertNTS_atI_def = Define`
+  insertNTS_atI (l1:word8 list) n l2 =
+    TAKE n l2 ++ l1 ++ [0w] ++ DROP (n + LENGTH l1 + 1) l2
 `;
 
-val CHAR_IO_def = Define`
-  CHAR_IO = CHAR_IO_char1 * CHAR_IO_fname
-`;
+val insertNTS_atI_NIL = Q.store_thm(
+  "insertNTS_atI_NIL",
+  `∀n l. n < LENGTH l ==> insertNTS_atI [] n l = LUPDATE 0w n l`,
+  simp[insertNTS_atI_def] >> Induct_on `n`
+  >- (Cases_on `l` >> simp[LUPDATE_def]) >>
+  Cases_on `l` >> simp[LUPDATE_def, ADD1]);
 
-val write_spec = store_thm ("write_spec",
-  ``!c cv.
-     WORD (c:word8) cv ==>
-     app (p:'ffi ffi_proj) ^(fetch_v "CharIO.write" (basis_st()))
-       [cv]
-       (CHAR_IO * CATFS fs)
-       (POSTv uv. cond (UNIT_TYPE () uv) * CHAR_IO * CATFS (fs with stdout := fs.stdout ++ [CHR (w2n c)]))``,
-  xcf "CharIO.write" (basis_st())
-  \\ fs [CHAR_IO_def, CHAR_IO_char1_def] \\ xpull
-  \\ xlet `POSTv zv. CATFS fs * W8ARRAY onechar_loc [c] * CHAR_IO_fname *
-                     & (UNIT_TYPE () zv)`
-  THEN1
-   (xapp \\ xsimpl \\ fs [EVAL ``onechar_loc``]
-    \\ instantiate \\ xsimpl \\ EVAL_TAC)
-  \\ xlet `POSTv _. CATFS (fs with stdout := fs.stdout ++ [CHR (w2n c)]) * W8ARRAY onechar_loc [c] * CHAR_IO_fname`
-  THEN1
-   (xffi
-    \\ simp [EVAL ``onechar_loc``, CATFS_def]
-    \\ `MEM 0 [0n;1;2;3]` by EVAL_TAC \\ instantiate \\ xsimpl
-    \\ simp[write_lemma])
-  \\ xret \\ xsimpl);
+val insertNTS_atI_CONS = Q.store_thm(
+  "insertNTS_atI_CONS",
+  `∀n l h t.
+     n + LENGTH t + 1 < LENGTH l ==>
+     insertNTS_atI (h::t) n l = LUPDATE h n (insertNTS_atI t (n + 1) l)`,
+  simp[insertNTS_atI_def] >> Induct_on `n`
+  >- (Cases_on `l` >> simp[ADD1, LUPDATE_def]) >>
+  Cases_on `l` >> simp[ADD1] >> fs[ADD1] >>
+  simp[GSYM ADD1, LUPDATE_def]);
 
-(*
-val open_spec = Q.store_thm(
-  "open_spec",
-  ``∀fnm
-
-val e =
-  ``LetApps "_" (Long "CharIO" "write") [Lit (Word8 (n2w (ORD #"H")))]
-      (LetApps "_" (Long "CharIO" "write") [Lit (Word8 (n2w (ORD #"i")))]
-         (Var (Short "_")))`` |> EVAL |> concl |> rand
-
-val _ = ml_prog_update (add_Dlet_Fun ``"main"`` ``"c"`` e "main_v")
-
-val main_spec = store_thm ("main",
-  ``!cv input output.
-      app (p:'ffi ffi_proj) ^(fetch_v "main" (basis_st()))
-        [cv]
-        (CHAR_IO * STDOUT "")
-        (POSTv uv. CHAR_IO * STDOUT "Hi")``,
-  xcf "main" (basis_st())
-  \\ xlet `POSTv v. CHAR_IO * STDOUT "H"` THEN1
-   (xapp \\ qexists_tac `emp` \\ qexists_tac `""` \\ qexists_tac `n2w (ORD #"H")`
-    \\ xsimpl)
-  \\ xlet `POSTv v. CHAR_IO * STDOUT "Hi"` THEN1
-   (xapp \\ qexists_tac `emp` \\ qexists_tac `"H"` \\ qexists_tac `n2w (ORD #"i")`
-    \\ xsimpl)
-  \\ xvar \\ fs [] \\ xsimpl);
-
-val main_applied = let
-  val e = ``Apps [Var (Short "main"); Lit (IntLit 0)] ``
-          |> EVAL |> concl |> rand
-  val th = get_ml_prog_state () |> get_thm
-  val th = MATCH_MP ml_progTheory.ML_code_NONE_Dlet_var th
-           handle HOL_ERR _ =>
-           MATCH_MP ml_progTheory.ML_code_SOME_Dlet_var th
-  val goal = th |> SPEC e |> SPEC_ALL |> concl |> dest_imp |> fst
-  val th = goal |> NCONV 6 (SIMP_CONV (srw_ss())
-                    [Once bigStepTheory.evaluate_cases,PULL_EXISTS])
-  val p = find_term (can (match_term ``lookup_var_id _ _ = SOME _``)) (concl th)
-  val th = th |> SIMP_RULE std_ss [EVAL p]
-  val exists_lemma = METIS_PROVE []
-    ``(?x1 x2 x3 x4 x5 x6. P x1 x2 x3 x4 x5 x6) <=>
-      (?x3 x4 x5 x6 x1 x2. P x1 x2 x3 x4 x5 x6)``
-  val st = goal |> rator |> rator |> rand
-  val th =
-    main_spec |> SPEC_ALL |> Q.INST_TYPE [`:'ffi`|->`:'a`]
-     |> REWRITE_RULE [cfAppTheory.app_basic_rel,cfAppTheory.app_def]
-     |> Q.SPEC `st2heap (p:'a ffi_proj) ^st`
-     |> Q.SPEC `{}`
-     |> Q.SPEC `^st`
-     |> SIMP_RULE std_ss [PULL_EXISTS,
-          cfHeapsBaseTheory.res_case_def,
-          cfHeapsBaseTheory.POSTv_ignore,
-          cfHeapsBaseTheory.SPLIT3_emp3,
-          cfHeapsBaseTheory.SPLIT_emp2]
-     |> Q.INST [`cv`|->`Litv (IntLit 0)`]
-     |> SIMP_RULE std_ss [Once exists_lemma]
-     |> SIMP_RULE std_ss [GSYM PULL_EXISTS,GSYM th]
-  in th end
-
-val raw_evaluate_prog = let
-  val th = get_ml_prog_state () |> get_thm
-  val th = MATCH_MP ml_progTheory.ML_code_NONE_Dlet_var th
-  val th = th |> SPEC_ALL |> UNDISCH |> Q.SPEC `"_"` |> DISCH_ALL |> GEN_ALL
-  val th = ConseqConv.WEAKEN_CONSEQ_CONV_RULE
-             (ConseqConv.CONSEQ_REWRITE_CONV ([],[],[th])) main_applied
-  val tm = th |> concl |> find_term (listSyntax.is_snoc)
-  val entire_program_def = Define `entire_program = ^tm`
-  val th = th |> SIMP_RULE std_ss [GSYM entire_program_def,PULL_EXISTS,
-                   ml_progTheory.ML_code_def,ml_progTheory.Prog_def]
-  in th end
-
-*)
-val _ = export_theory();
+val _ = export_theory()
